\begin{subequations}
\begin{equation}
\begin{cases}
\left.\partial_z \theta \right|_{\rm top} =
\left.\partial_z u \right|_{\rm top} = 0& \\
\left(\partial_t - \partial_z (K_\theta \partial_z )\right)
\theta = 0 , ~~~~~&
\left(\partial_t + if - \partial_z (K_u \partial_z )\right)
u =  i f u_G \\
\left. K_\theta \partial_z \theta \right|_{{\delta_a}}
= C_H |u_a - u_o| (\theta_a - \theta_o), ~~~~~&
\left. K_u \partial_z u \right|_{{\delta_a}}
= \frac{{(u^\star_a)}^2}{|u_a - u_o|} (u_a - u_o)
\end{cases}
\end{equation}
\begin{equation}
u^\star_a, \theta^\star_a, u^\star_o, \theta^\star_o =
{\rm BULK}(u_a, u_o,
\theta_a, \theta_o, \delta_a, \delta_o, Q_{lw}, Q_{sw})
\end{equation}
\begin{equation}
\begin{cases}
\left. K_\theta \partial_z \theta \right|_{\delta_o}
= u^\star_o \theta^\star_o +
\frac{Q_{lw} + Q_{sw}(\delta_o)}{\rho_0 c_p},
~~~~~&
\left. K_u \partial_z u \right|_{{\delta_o}}
= \frac{{(u^\star_o)}^2}{|u_a - u_o|} (u_a - u_o) \\
\left(\partial_t - \partial_z (K_\theta \partial_z )\right)
\theta = \frac{\partial_z Q_{sw}}{\rho_0 c_p} , ~~~~~&
\left(\partial_t + if - \partial_z (K_u \partial_z )\right)
u =  0 \\
\left.\partial_z \theta \right|_{\rm bottom} =
\left.\partial_z u \right|_{\rm bottom} = 0&
\end{cases}
\end{equation}
\end{subequations}
